checkpointing to share with Yi

lib/Lang/System/PackedInts.s.dfy
@@ -9,7 +9,51 @@ abstract module NativePackedInt {
 
   function method Size() : uint64
     ensures 0 < Size()
+
+  function MinValue() : int
+    ensures MinValue() <= 0
+  function UpperBound() : int
+    ensures MinValue() < UpperBound()
+
+  // These exist because there's no way to promise dafny that Integer is an int type.
+  function fromInt(x: int) : (result: Integer)
+    requires MinValue() <= x < UpperBound()
+  function toInt(x: Integer) : (result: int)
+    ensures MinValue() <= result < UpperBound()
+    ensures fromInt(result) == x
+  predicate method fitsInInteger(x: uint64)
+  function method fromUint64(x: uint64) : (result: Integer)
+    requires MinValue() <= x as int < UpperBound()
+    ensures result == fromInt(x as nat)
+  predicate method fitsInUint64(x: Integer)
+    ensures fitsInUint64(x) <==> 0 <= toInt(x) < 0x1_0000_0000_0000_0000
+  function method toUint64(x: Integer) : (result: uint64)
+    requires 0 <= toInt(x) < 0x1_0000_0000_0000_0000
+    ensures MinValue() <= result as int < UpperBound()
+    ensures result as int == toInt(x)
+
+  function {:opaque} fromIntSeq(s: seq<int>) : (result: seq<Integer>)
+    requires forall i | 0 <= i < |s| :: fromInt.requires(s[i])
+    ensures |result| == |s|
+    ensures forall i | 0 <= i < |result| :: result[i] == fromInt(s[i])
+  {
+    if s == [] then
+      []
+    else
+      fromIntSeq(s[..|s|-1]) + [ fromInt(s[|s|-1]) ]
+  }
     
+  function {:opaque} toIntSeq(s: seq<Integer>) : (result: seq<int>)
+    requires forall i | 0 <= i < |s| :: toInt.requires(s[i])
+    ensures |result| == |s|
+    ensures forall i | 0 <= i < |result| :: result[i] == toInt(s[i])
+  {
+    if s == [] then
+      []
+    else
+      toIntSeq(s[..|s|-1]) + [ toInt(s[|s|-1]) ]
+  }
+
   function unpack(s: seq<byte>) : Integer
     requires |s| == Size() as nat
 
@@ -59,9 +103,26 @@ module NativePackedByte refines NativePackedInt{
   type Integer = byte
     
   function method Size() : uint64 { 1 }
-    
-  function {:opaque} unpack(s: seq<byte>) : Integer
-  {
+  function MinValue() : int { 0 }
+  function UpperBound() : int { 0x100 }
+  
+  function fromInt(x: int) : (result: Integer) {
+    x as byte
+  }
+  
+  function toInt(x: Integer) : int {
+    x as int
+  }
+
+  function method fromUint64(x: uint64) : (result: Integer) {
+    x as byte
+  }
+  
+  function method toUint64(x: Integer) : uint64 {
+    x as uint64
+  }
+  
+  function {:opaque} unpack(s: seq<byte>) : Integer {
     s[0]
   }
 
@@ -74,10 +135,27 @@ module NativePackedByte refines NativePackedInt{
 module NativePackedUint32 refines NativePackedInt{
   type Integer = uint32
 
+  function MinValue() : int { 0 }
+  function UpperBound() : int { 0x1_0000_0000 }
   function method Size() : uint64 { 4 }
     
-  function {:opaque} unpack(s: seq<byte>) : Integer
-  {
+  function fromInt(x: int) : (result: Integer) {
+    x as uint32
+  }
+
+  function toInt(x: Integer) : int {
+    x as int
+  }
+
+  function method fromUint64(x: uint64) : (result: Integer) {
+    x as uint32
+  }
+  
+  function method toUint64(x: Integer) : uint64 {
+    x as uint64
+  }
+  
+  function {:opaque} unpack(s: seq<byte>) : Integer {
     (s[0] as uint32)
     + (s[1] as uint32 * 0x1_00)
     + (s[2] as uint32 * 0x1_00_00)
@@ -93,8 +171,26 @@ module NativePackedUint32 refines NativePackedInt{
 module NativePackedUint64 refines NativePackedInt{
   type Integer = uint64
 
+  function MinValue() : int { 0 }
+  function UpperBound() : int { 0x1_0000_0000_0000_0000 }
   function method Size() : uint64 { 8 }
     
+  function fromInt(x: int) : (result: Integer) {
+    x as uint64
+  }
+
+  function toInt(x: Integer) : int {
+    x as int
+  }
+
+  function method fromUint64(x: uint64) : (result: Integer) {
+    x
+  }
+  
+  function method toUint64(x: Integer) : uint64 {
+    x
+  }
+  
   function {:opaque} unpack(s: seq<byte>) : Integer
   {
     (s[0] as uint64)
